core/HeisenbergLight.v
@@ -1,0 +1,263 @@
+Require Import QWIRE.Prelim.
+Require Import SQIR.
+
+(* The Clifford Set of Unitary Matrices *)
+Inductive Clifford : nat -> Set := 
+  | U_H                  : Clifford 1 
+  | U_S                  : Clifford 1 
+  | U_CNOT               : Clifford 2.
+
+Definition clifford_ucom := ucom Clifford.
+
+Local Open Scope ucom.
+
+(* Some useful shorthands. *)
+Definition CNOT {dim} m n : clifford_ucom dim := uapp2 U_CNOT m n.  
+Definition H {dim} n : clifford_ucom dim := uapp1 U_H n.  
+Definition S {dim} n : clifford_ucom dim := uapp1 U_S n.  
+Definition Z {dim} n : clifford_ucom dim := S n ; S n.
+Definition X {dim} n : clifford_ucom dim := H n; Z n; H n. 
+(* Y = iXZ *)
+(* Definition Y {dim} n : clifford_ucom dim := X n; Z n. *)
+Definition I {dim} n : clifford_ucom dim := H n; H n. 
+Definition CZ {dim} m n : clifford_ucom dim :=
+  H n ; CNOT m n ; H n.
+Definition SWAP {dim} m n : clifford_ucom dim :=
+  CNOT m n; CNOT n m; CNOT m n.
+
+Inductive htype : Set := II | XX | YY | ZZ.
+
+(* From Gottesman, table 1 *)
+Definition apply1 (c : Clifford 1) (b : htype) : htype :=
+  match c, b with 
+  | U_H, II => II (* noop *)
+  | U_H, XX => ZZ
+  | U_H, YY => YY (* inferred *)
+  | U_H, ZZ => XX
+  | U_S, II => II (* noop *)
+  | U_S, XX => YY
+  | U_S, YY => XX (* inferred *)
+  | U_S, ZZ => ZZ
+  end.
+
+(* CNOT (h ⊗ II) *)
+Definition apply_cnot1 (h : htype) : htype * htype :=
+  match h with
+  | II => (II, II)
+  | XX => (XX, XX)
+  | ZZ => (ZZ, II)
+  | YY => (YY, XX) (* inferred *)
+  end.
+           
+(* CNOT (II ⊗ h) *)
+Definition apply_cnot2 (h : htype) : htype * htype :=
+  match h with
+  | II => (II, II)
+  | XX => (II, XX)
+  | ZZ => (ZZ, ZZ)
+  | YY => (ZZ, YY) (* inferred *)
+  end.
+
+Definition h_times (h1 h2 : htype) :=
+  match h1, h2 with
+  | II, h2 => h2
+  | h1, II => h1
+  | XX, XX => II
+  | XX, YY => ZZ
+  | XX, ZZ => YY
+  | YY, XX => ZZ
+  | YY, YY => II
+  | YY, ZZ => XX
+  | ZZ, XX => YY
+  | ZZ, YY => XX
+  | ZZ, ZZ => II
+  end.
+
+Infix "*" := h_times.
+
+Definition apply_cnot (h1 h2 : htype) : htype * htype :=
+  let (h11, h12) := apply_cnot1 h1 in                
+  let (h21, h22) := apply_cnot2 h2 in
+  (h11 * h21, h12 * h22).
+
+(* Belongs in Prelim -- and Coq standard lib *)
+Lemma fold_if : forall (b : bool), (if b then true else false) = b.
+Proof. destruct b; easy. Qed.
+
+Lemma II_1_l : forall h, II * h = h.
+Proof. reflexivity. Qed.
+
+Lemma II_1_r : forall h, h * II = h.
+Proof. intros []; reflexivity. Qed.
+
+Lemma h_times_inv : forall h, h * h = II.
+Proof. intros []; reflexivity. Qed.
+
+Example CNOT_IX : apply_cnot II XX = (II, XX).
+Proof. reflexivity. Qed.
+Example CNOT_XI : apply_cnot XX II = (XX, XX).
+Proof. reflexivity. Qed.
+Example CNOT_IZ : apply_cnot II ZZ = (ZZ, ZZ).
+Proof. reflexivity. Qed.
+Example CNOT_ZI : apply_cnot ZZ II = (ZZ, II).
+Proof. reflexivity. Qed.
+Example CNOT_XX : apply_cnot XX XX = (XX, II).
+Proof. reflexivity. Qed.
+
+Definition h_state := list htype. 
+
+Definition all_X_state (dim : nat) := repeat XX dim.
+Definition all_Y_state (dim : nat) := repeat YY dim.
+Definition all_Z_state (dim : nat) := repeat ZZ dim.
+Definition all_I_state (dim : nat) := repeat II dim. (* should never appear *)
+
+(*
+Fixpoint apply_at {A} (f : A -> A) (i : nat) (l : list A) : list A :=
+  match l, i with
+  | [], _                  => []
+  | a :: l', 0              => f a :: l'
+  | a :: l', Datatypes.S i' => a :: apply_at f i' l' 
+  end.
+*)
+
+Notation "[ ]" := nil (format "[ ]") : list_scope.
+Notation "[ x ]" := (cons x nil) : list_scope.
+Notation "[ x , y , .. , z ]" := (cons x (cons y .. (cons z nil) ..)) : list_scope.
+
+Fixpoint count {A} (f : A -> bool) (l : list A) : nat :=
+  match l with
+  | [] => 0
+  | a :: l' => if f a then 1 + (count f l') else count f l'
+  end. 
+
+Fixpoint h_eval {dim} (c : clifford_ucom dim) (st : h_state) : h_state :=
+  match c with
+  | c1 ; c2      => h_eval c2 (h_eval c1 st)
+  | uapp1 U n    => update_at st n (apply1 U (nth n st II)) 
+  | uapp2 _ m n  => let (h1,h2) := apply_cnot (nth m st II) (nth n st II) in
+                   update_at (update_at st m h1) n h2
+  | _            => all_I_state dim (* no 3-qubit gates in our denotation function *) 
+  end.
+  
+(** * Examples from Gottesman Paper *)
+
+(* Example 1 *)
+
+Lemma SWAP_X1 : h_eval (@SWAP 2 0 1) [XX,II] = [II,XX].
+Proof. reflexivity. Qed.
+
+Lemma SWAP_basis : forall (h1 h2 : htype),
+ h_eval (@SWAP 2 0 1) [h1,h2] = [h2,h1].
+Proof. intros [] []; subst; reflexivity. Qed.
+
+(* Could reduce to a two case proof and add a proof that this is
+   sufficient to reason about all cases.  *)
+
+(* Example 2 *)
+
+Definition had_cnot : clifford_ucom 2 := 
+  H 0; H 1; CNOT 0 1; H 0; H 1.
+
+Lemma had_cnot_notc : forall (h1 h2 : htype),
+  h_eval had_cnot [h1,h2] = h_eval (@CNOT 2 1 0) [h1,h2].   
+Proof. intros [] []; reflexivity. Qed.
+
+(* TODO: Want a general notion of equality between programs. *)
+
+(* Example 3 *)
+
+Definition hitite_code : clifford_ucom 2 := 
+  H 0; S 1; CNOT 0 1; H 1; CNOT 0 1.
+
+Lemma hitite_X1 : h_eval hitite_code [XX,II] = [ZZ,II].
+Proof. reflexivity. Qed.
+
+(* Gottesman puts the negation in from of the II *)
+Lemma hitite_X2 : h_eval hitite_code [II,XX] = [II, YY].
+Proof. reflexivity. Qed.
+
+(* Gottesman uses [-YY,YY] *)
+Lemma hitite_Z1 : h_eval hitite_code [ZZ,II] = [YY, YY].
+Proof. reflexivity. Qed.
+
+Lemma hitite_Z2 : h_eval hitite_code [II,ZZ] = [ZZ, XX].
+Proof. reflexivity. Qed.
+
+(* Example 4 *)
+
+Definition cnot_notc : clifford_ucom 2 := CNOT 0 1; CNOT 1 0.
+
+(* unlabelled case *)
+Lemma cnot_notc_Z2 : h_eval cnot_notc [II,ZZ] = [ZZ,II].
+Proof. reflexivity. Qed.
+
+Lemma cnot_notc_X1 : h_eval cnot_notc [XX,II] = [II,XX].
+Proof. reflexivity. Qed.
+
+Lemma cnot_notc_Z1 : h_eval cnot_notc [ZZ,II] = [ZZ,ZZ].
+Proof. reflexivity. Qed.
+
+(* Example 5 *)
+
+Definition bell : clifford_ucom 2 := H 0; CNOT 0 1.
+
+Lemma bell_Z1 : h_eval bell [ZZ,II] = [XX,XX].
+Proof. reflexivity. Qed.
+
+Lemma bell_Z2 : h_eval bell [II,ZZ] = [ZZ,ZZ].
+Proof. reflexivity. Qed.
+
+(* Example 6 *)
+
+(* Can we represent this as a program? *)
+
+(* Example 7 *)
+
+Definition ec_code : clifford_ucom 4 := 
+  H 3; CNOT 0 2; CNOT 1 2; CNOT 3 0; CNOT 3 1; CNOT 3 2.
+
+(* What to prove? *)
+
+(* Example 8 *)
+
+(* Example 9 *)
+
+(* Now with measurement! *)
+
+(* Example 10: Teleportation *)
+
+(* Measurement-free teleportation with bell initialization *)
+
+Definition bell' : clifford_ucom 3 := H 1; CNOT 1 2.
+
+Definition alice : clifford_ucom 3 := CNOT 0 1; H 0.
+
+Definition bob : clifford_ucom 3 := CNOT 1 2; CZ 0 2.
+
+Definition teleport : clifford_ucom 3 := bell'; alice; bob.
+
+Lemma alice_X1 : h_eval alice [XX,II,II] = [ZZ,XX,II].
+Proof. reflexivity. Qed.
+
+Lemma alice_Z1 : h_eval alice [ZZ,II,II] = [XX,II,II].
+Proof. reflexivity. Qed.
+
+Lemma bob_X1 : h_eval bob [ZZ,XX,II] = [II,XX,XX].
+Proof. reflexivity. Qed.
+
+Lemma bob_Z1 : h_eval bob [XX,II,II] = [XX,II,ZZ].
+Proof. reflexivity. Qed.
+
+Lemma teleport_X1 : h_eval teleport [XX,II,II] = [II,XX,XX].
+Proof. simpl. reflexivity. Qed.
+
+Lemma teleport_Z1 : h_eval teleport [ZZ,II,II] = [XX,II,ZZ].
+Proof. simpl. reflexivity. Qed.
+
+(* Example 11: Remove XOR *)
+
+
+(** Own examples *)
+
+(* GHZ state *)
+
